Orderedtree/DOrderedTree/Internal/Impl/Balancing.lean
@@ -1,0 +1,488 @@
+/-
+Copyright (c) 2024 Lean FRO, LLC. All rights reserved.
+Released under Apache 2.0 license as described in the file LICENSE.
+Authors: Markus Himmel
+-/
+import Orderedtree.Classes.LawfulEqOrd
+import Orderedtree.DOrderedTree.Internal.Impl.Attr
+import Orderedtree.Classes.TransOrd
+import Lean.Elab.Tactic
+
+/-!
+# Low-level implementation of the size-bounded tree
+
+This file contains the basic definition implementing the functionality of the size-bounded trees.
+-/
+
+set_option autoImplicit false
+set_option linter.all true
+
+universe u v w
+
+variable {α : Type u} {β : α → Type v} {γ : α → Type w} {δ : Type w} {m : Type w → Type w}
+
+namespace Std.DOrderedTree.Internal
+
+/-- Predicate for local balance at a node of the tree. We don't provide API for this, preferring
+instead to use automation to dispatch goals about balance. -/
+@[tree_tac]
+def BalancedAtRoot (left right : Nat) : Prop :=
+  left + right ≤ 1 ∨ (left ≤ delta * right ∧ right ≤ delta * left)
+
+/-- Predicate that states that the stored size information in a tree is correct and that it is
+balanced. -/
+inductive Balanced : Impl α β → Prop where
+  /-- Leaf is balanced. -/
+  | leaf : Balanced leaf
+  /-- Inner node is balanced if it is locally balanced, both children are balanced and size
+  information is correct. -/
+  | inner {sz k v l r} : Balanced l → Balanced r →
+      BalancedAtRoot l.size r.size → sz = l.size + 1 + r.size → Balanced (inner sz k v l r)
+
+attribute [tree_tac] Balanced.leaf
+
+@[tree_tac]
+theorem balanced_inner_iff {sz k v l r} : Balanced (Impl.inner sz k v l r : Impl α β) ↔
+    Balanced l ∧ Balanced r ∧ BalancedAtRoot l.size r.size ∧ sz = l.size + 1 + r.size :=
+  ⟨by rintro (_|⟨h₁, h₂, h₃, h₄⟩); exact ⟨h₁, h₂, h₃, h₄⟩,
+   fun ⟨h₁, h₂, h₃, h₄⟩ => .inner h₁ h₂ h₃ h₄⟩
+
+/-!
+## Balancing operations
+-/
+
+/-- Precondition for `balanceL`: at most one element was added to left subtree. -/
+@[tree_tac]
+abbrev BalanceLPrecond (left right : Nat) :=
+  BalancedAtRoot left right ∨ (1 ≤ left ∧ BalancedAtRoot (left - 1) right)
+
+/-- Precondition for `balanceLErase`. As Breitner et al. remark, "not very educational". -/
+@[tree_tac]
+abbrev BalanceLErasePrecond (left right : Nat) :=
+  (delta * left ≤ delta * delta * right + delta * right + right + delta ∧ right + 1 ≤ left) ∨
+    BalancedAtRoot left (right + 1) ∨ BalancedAtRoot left right
+
+section
+
+open Lean Meta Elab Tactic
+
+/-- (Implementation detail) -/
+elab "as_aux_lemma" " => " s:tacticSeq : tactic => liftMetaTactic fun mvarId => do
+  let (mvars, _) ← runTactic mvarId s
+  unless mvars.isEmpty do
+    throwError "Left-over goals, cannot abstract"
+  let e ← instantiateMVars (mkMVar mvarId)
+  let e ← mkAuxTheorem (`Std.DOrderedTree.Internal.Impl ++ (← mkFreshUserName `test)) (← mvarId.getType) e
+  mvarId.assign e
+  return []
+
+/-- (Implementation detail) -/
+scoped macro "tree_tac" : tactic => `(tactic|(
+  subst_eqs
+  repeat' split
+  all_goals
+    try simp only [tree_tac] at *
+  all_goals
+    try simp only [tree_tac] at *
+    repeat cases ‹_ ∧ _›
+    repeat' apply And.intro
+  all_goals
+    try assumption
+    try contradiction
+  all_goals
+    subst_eqs
+    omega
+  ))
+
+/-- (Implementation detail) -/
+scoped macro "✓" : term => `(term| by as_aux_lemma => tree_tac)
+
+end
+
+theorem BalanceLPrecond.erase {left right : Nat} :
+    BalanceLPrecond left right → BalanceLErasePrecond left right := by
+  tree_tac
+
+/-!
+### `balanceL` variants
+-/
+
+/-- Rebalances a tree after at most one element was added to the left subtree. Uses balancing
+information to show that some cases are impossible. -/
+@[inline]
+def balanceL (k : α) (v : β k) (l r : Impl α β) (hlb : Balanced l) (hrb : Balanced r)
+    (hlr : BalanceLPrecond l.size r.size) : Impl α β :=
+  match r with
+  | leaf => match l with
+    | leaf => .inner 1 k v .leaf .leaf
+    | inner _ _ _ .leaf .leaf => .inner 2 k v l .leaf
+    | inner _ lk lv .leaf (.inner _ lrk lrv _ _) =>
+        .inner 3 lrk lrv (.inner 1 lk lv .leaf .leaf) (.inner 1 k v .leaf .leaf)
+    | inner _ lk lv ll@(.inner _ _ _ _ _) .leaf =>
+        .inner 3 lk lv ll (.inner 1 k v .leaf .leaf)
+    | inner ls lk lv (.inner lls _ _ _ _) (.inner lrs _ _ _ _) => False.elim ✓
+  | inner rs _ _ _ _ => match l with
+    | leaf => .inner (1 + rs) k v .leaf r
+    | inner ls lk lv ll lr =>
+        if hlsd : delta * rs < ls then match ll, lr with
+          | inner lls _ _ _ _, inner lrs lrk lrv lrl lrr =>
+              if lrs < ratio * lls then
+                .inner (1 + ls + rs) lk lv ll (.inner (1 + rs + lrs) k v (inner lrs lrk lrv lrl lrr) r)
+              else
+                .inner (1 + ls + rs) lrk lrv (.inner (1 + lls + lrl.size) lk lv ll lrl)
+                  (.inner (1 + rs + lrr.size) k v lrr r)
+          | inner _ _ _ _ _, leaf => False.elim ✓
+          | leaf, _ => False.elim ✓
+        else .inner (1 + ls + rs) k v (.inner ls lk lv ll lr) r
+
+/-- Slower version of `balanceL` with weaker balancing assumptions that hold after erasing from
+the right side of the tree. -/
+@[inline]
+def balanceLErase (k : α) (v : β k) (l r : Impl α β) (hlb : Balanced l) (hrb : Balanced r)
+    (hlr : BalanceLErasePrecond l.size r.size) : Impl α β :=
+  match r with
+  | leaf => match l with
+    | leaf => .inner 1 k v .leaf .leaf
+    | inner _ _ _ .leaf .leaf => .inner 2 k v l .leaf
+    | inner _ lk lv .leaf (.inner _ lrk lrv _ _) =>
+        .inner 3 lrk lrv (.inner 1 lk lv .leaf .leaf) (.inner 1 k v .leaf .leaf)
+    | inner _ lk lv ll@(.inner _ _ _ _ _) .leaf =>
+        .inner 3 lk lv ll (.inner 1 k v .leaf .leaf)
+    | inner ls lk lv ll@(.inner lls _ _ _ _) lr@(.inner lrs lrk lrv lrl lrr) =>
+        .inner (1 + ls) lk lv ll (.inner (1 + lrs) k v lr .leaf)
+  | (inner rs _ _ _ _) => match l with
+    | leaf => .inner (1 + rs) k v .leaf r
+    | (inner ls lk lv ll lr) =>
+        if hlsd : delta * rs < ls then match ll, lr with
+          | inner lls _ _ _ _, inner lrs lrk lrv lrl lrr =>
+              if lrs < ratio * lls then
+                .inner (1 + ls + rs) lk lv ll (.inner (1 + rs + lrs) k v lr r)
+              else
+                .inner (1 + ls + rs) lrk lrv (.inner (1 + lls + lrl.size) lk lv ll lrl)
+                  (.inner (1 + rs + lrr.size) k v lrr r)
+          | inner _ _ _ _ _, leaf => False.elim ✓
+          | leaf, _ => False.elim ✓
+        else .inner (1 + ls + rs) k v l r
+
+/-- Slow version of `balanceL` which can be used in the complete absence of balancing information
+but still assumes that the preconditions of `balanceL` or `balanceL` are satisfied
+(otherwise panics). -/
+@[inline] def balanceLSlow (k : α) (v : β k) (l r : Impl α β) : Impl α β :=
+  match r with
+  | leaf => match l with
+    | leaf => .inner 1 k v .leaf .leaf
+    | inner _ _ _ .leaf .leaf => .inner 2 k v l .leaf
+    | inner _ lk lv .leaf (.inner _ lrk lrv _ _) =>
+        .inner 3 lrk lrv (.inner 1 lk lv .leaf .leaf) (.inner 1 k v .leaf .leaf)
+    | inner _ lk lv ll@(.inner _ _ _ _ _) .leaf =>
+        .inner 3 lk lv ll (.inner 1 k v .leaf .leaf)
+    | inner ls lk lv ll@(.inner _ _ _ _ _) lr@(.inner lrs _ _ _ _) =>
+        .inner (1 + ls) lk lv ll (.inner (1 + lrs) k v lr .leaf)
+  | (inner rs _ _ _ _) => match l with
+    | leaf => .inner (1 + rs) k v .leaf r
+    | inner ls lk lv ll lr =>
+        if ls > delta * rs then match ll, lr with
+          | inner lls _ _ _ _, inner lrs lrk lrv lrl lrr =>
+              if lrs < ratio * lls then
+                .inner (1 + ls + rs) lk lv ll (.inner (1 + rs + lrs) k v lr r)
+              else
+                .inner (1 + ls + rs) lrk lrv (.inner (1 + lls + lrl.size) lk lv ll lrl)
+                  (.inner (1 + rs + lrr.size) k v lrr r)
+          | inner _ _ _ _ _, leaf => panic! "balanceLSlow input was not balanced"
+          | leaf, _ => panic! "balanceLSlow input was not balanced"
+        else .inner (1 + ls + rs) k v l r
+
+/-!
+### `balanceR` variants
+-/
+
+/-- Rebalances a tree after at most one element was added to the right subtree. Uses balancing
+information to show that some cases are impossible. -/
+@[inline]
+def balanceR (k : α) (v : β k) (l r : Impl α β) (hlb : Balanced l) (hrb : Balanced r)
+    (hlr : BalanceLPrecond r.size l.size) : Impl α β :=
+  match l with
+  | leaf => match r with
+    | leaf => .inner 1 k v .leaf .leaf
+    | (inner _ _ _ .leaf .leaf) => .inner 2 k v .leaf r
+    | inner _ rk rv .leaf rr@(.inner _ _ _ _ _) => .inner 3 rk rv (.inner 1 k v .leaf .leaf) rr
+    | inner _ rk rv (.inner _ rlk rlv _ _) .leaf => .inner 3 rlk rlv (.inner 1 k v .leaf .leaf)
+        (.inner 1 rk rv .leaf .leaf)
+    | inner rs rk rv (.inner rls rlk rlv rll rlr) (.inner rrs _ _ _ _) =>
+        False.elim ✓
+  | inner ls _ _ _ _ => match r with
+    | leaf => .inner (1 + ls) k v l .leaf
+    | inner rs rk rv rl rr =>
+        if hrsd : rs > delta * ls then match rl, rr with
+          | inner rls rlk rlv rll rlr, .inner rrs _ _ _ _ =>
+              if rls < ratio * rrs then
+                .inner (1 + ls + rs) rk rv (.inner (1 + ls + rls) k v l (.inner rls rlk rlv rll rlr)) rr
+              else
+                .inner (1 + ls + rs) rlk rlv (.inner (1 + ls + rll.size) k v l rll)
+                  (.inner (1 + rrs + rlr.size) rk rv rlr rr)
+          | inner _ _ _ _ _, leaf => False.elim ✓
+          | leaf, _ => False.elim ✓
+        else .inner (1 + ls + rs) k v l (inner rs rk rv rl rr)
+
+/-- Slower version of `balanceR` with weaker balancing assumptions that hold after erasing from
+the left side of the tree. -/
+@[inline]
+def balanceRErase (k : α) (v : β k) (l r : Impl α β) (hlb : Balanced l) (hrb : Balanced r)
+    (hlr : BalanceLErasePrecond r.size l.size) : Impl α β :=
+  match l with
+  | leaf => match r with
+    | leaf => .inner 1 k v .leaf .leaf
+    | r@(inner _ _ _ .leaf .leaf) => .inner 2 k v .leaf r
+    | inner _ rk rv .leaf rr@(.inner _ _ _ _ _) => .inner 3 rk rv (.inner 1 k v .leaf .leaf) rr
+    | inner _ rk rv (.inner _ rlk rlv _ _) .leaf => .inner 3 rlk rlv (.inner 1 k v .leaf .leaf)
+        (.inner 1 rk rv .leaf .leaf)
+    | inner rs rk rv rl@(.inner rls rlk rlv rll rlr) rr@(.inner rrs _ _ _ _) =>
+        .inner (1 + rs) rk rv (.inner (1 + rls) k v .leaf rl) rr
+  | inner ls _ _ _ _ => match r with
+    | leaf => .inner (1 + ls) k v l .leaf
+    | inner rs rk rv rl rr =>
+        if hrsd : rs > delta * ls then match rl, rr with
+          | inner rls rlk rlv rll rlr, .inner rrs _ _ _ _ =>
+              if rls < ratio * rrs then
+                .inner (1 + ls + rs) rk rv (.inner (1 + ls + rls) k v l rl) rr
+              else
+                .inner (1 + ls + rs) rlk rlv (.inner (1 + ls + rll.size) k v l rll)
+                  (.inner (1 + rrs + rlr.size) rk rv rlr rr)
+          | inner _ _ _ _ _ , leaf => False.elim ✓
+          | leaf, _ => False.elim ✓
+        else .inner (1 + ls + rs) k v l r
+
+/-- Slow version of `balanceR` which can be used in the complete absence of balancing information
+but still assumes that the preconditions of `balanceR` or `balanceRErase` are satisfied
+(otherwise panics). -/
+@[inline]
+def balanceRSlow (k : α) (v : β k) (l r : Impl α β) : Impl α β :=
+  match l with
+  | leaf => match r with
+    | leaf => .inner 1 k v .leaf .leaf
+    | inner _ _ _ .leaf .leaf => .inner 2 k v .leaf r
+    | inner _ rk rv .leaf rr@(.inner _ _ _ _ _) => .inner 3 rk rv (.inner 1 k v .leaf .leaf) rr
+    | inner _ rk rv (.inner _ rlk rlv _ _) .leaf => .inner 3 rlk rlv (.inner 1 k v .leaf .leaf)
+        (.inner 1 rk rv .leaf .leaf)
+    | inner rs rk rv rl@(.inner rls _ _ _ _) rr@(.inner _ _ _ _ _) =>
+        .inner (1 + rs) rk rv (.inner (1 + rls) k v .leaf rl) rr
+  | inner ls _ _ _ _ => match r with
+    | leaf => .inner (1 + ls) k v l .leaf
+    | inner rs rk rv rl rr =>
+        if rs > delta * ls then match rl, rr with
+          | inner rls rlk rlv rll rlr, .inner rrs _ _ _ _ =>
+              if rls < ratio * rrs then
+                .inner (1 + ls + rs) rk rv (.inner (1 + ls + rls) k v l rl) rr
+              else
+                .inner (1 + ls + rs) rlk rlv (.inner (1 + ls + rll.size) k v l rll)
+                  (.inner (1 + rrs + rlr.size) rk rv rlr rr)
+          | inner _ _ _ _ _, leaf => panic! "balanceRSlow input was not balanced"
+          | leaf, _ => panic! "balanceRSlow input was not balanced"
+        else .inner (1 + ls + rs) k v l r
+
+/-!
+## `balance` variants
+-/
+
+/-- Rebalances a tree after at most one element was added or removed from either subtree. -/
+def balance (k : α) (v : β k) (l r : Impl α β) (hl : Balanced l) (hr : Balanced r)
+    (h : BalanceLErasePrecond l.size r.size ∨
+      BalanceLErasePrecond r.size l.size) : Impl α β :=
+  match l with
+  | .leaf =>
+    match r with
+    | .leaf => .inner 1 k v .leaf .leaf
+    | .inner _ _ _ .leaf .leaf => .inner 2 k v .leaf r
+    | .inner _ rk rv .leaf rr@(.inner _ _ _ _ _) => .inner 3 rk rv (.inner 1 k v .leaf .leaf) rr
+    | .inner _ rk rv (.inner _ rlk rlv _ _) .leaf => .inner 3 rlk rlv (.inner 1 k v .leaf .leaf)
+        (.inner 1 rk rv .leaf .leaf)
+    | .inner rs rk rv (.inner rls rlk rlv rll rlr) rr@(.inner rrs _ _ _ _) =>
+        .inner (1 + rs) rk rv (.inner (1 + rls) k v .leaf (.inner rls rlk rlv rll rlr)) rr
+  | .inner ls lk lv ll lr =>
+    match r with
+    | .leaf =>
+      match ll, lr with
+      | .leaf, .leaf => .inner 2 k v l .leaf
+      | .leaf, .inner _ lrk lrv _ _ => .inner 3 lrk lrv (.inner 1 lk lv .leaf .leaf)
+          (.inner 1 k v .leaf .leaf)
+      | .inner _ _ _ _ _, .leaf => .inner 3 lk lv ll (.inner 1 k v .leaf .leaf)
+      | .inner lls _ _ _ _, .inner lrs lrk lrv lrl lrr =>
+          .inner (1 + ls) lk lv ll (.inner (1 + lrs) k v (.inner lrs lrk lrv lrl lrr) .leaf)
+    | .inner rs rk rv rl rr =>
+      if h₁ : delta * ls < rs then
+        match rl, rr with
+        | .inner rls rlk rlv rll rlr, .inner rrs _ _ _ _ =>
+            if rls < ratio * rrs then
+              .inner (1 + ls + rs) rk rv (.inner (1 + ls + rls) k v l rl) rr
+            else
+              .inner (1 + ls + rs) rlk rlv (.inner (1 + ls + rll.size) k v l rll)
+                (.inner (1 + rrs + rlr.size) rk rv rlr rr)
+        | inner _ _ _ _ _, .leaf => False.elim ✓
+        | .leaf, _ => False.elim ✓
+      else if h₂ : delta * rs < ls then
+        match ll, lr with
+        | .inner lls _ _ _ _, .inner lrs lrk lrv lrl lrr =>
+            if lrs < ratio * lls then
+              .inner (1 + ls + rs) lk lv ll (.inner (1 + rs + lrs) k v lr r)
+            else
+              .inner (1 + ls + rs) lrk lrv (.inner (1 + lls + lrl.size) lk lv ll lrl)
+                (.inner (1 + rs + lrr.size) k v lrr r)
+        | inner _ _ _ _ _, .leaf => False.elim ✓
+        | .leaf, _ => False.elim ✓
+      else
+        .inner (1 + ls + rs) k v l r
+
+/-- Slow version of `balance` which can be used in the complete absence of balancing information
+but still assumes that the preconditions of `balance` are satisfied
+(otherwise panics). -/
+def balanceSlow (k : α) (v : β k) (l r : Impl α β) : Impl α β :=
+  match l with
+  | .leaf =>
+    match r with
+    | .leaf => .inner 1 k v .leaf .leaf
+    | .inner _ _ _ .leaf .leaf => .inner 2 k v .leaf r
+    | .inner _ rk rv .leaf rr@(.inner _ _ _ _ _) => .inner 3 rk rv (.inner 1 k v .leaf .leaf) rr
+    | .inner _ rk rv (.inner _ rlk rlv _ _) .leaf => .inner 3 rlk rlv (.inner 1 k v .leaf .leaf)
+        (.inner 1 rk rv .leaf .leaf)
+    | .inner rs rk rv (.inner rls rlk rlv rll rlr) rr@(.inner _ _ _ _ _) =>
+          .inner (1 + rs) rk rv (.inner (1 + rls) k v .leaf (.inner rls rlk rlv rll rlr)) rr
+  | .inner ls lk lv ll lr =>
+    match r with
+    | .leaf =>
+      match ll, lr with
+      | .leaf, .leaf => .inner 2 k v l .leaf
+      | .leaf, .inner _ lrk lrv _ _ => .inner 3 lrk lrv (.inner 1 lk lv .leaf .leaf)
+          (.inner 1 k v .leaf .leaf)
+      | .inner _ _ _ _ _, .leaf => .inner 3 lk lv ll (.inner 1 k v .leaf .leaf)
+      | .inner _ _ _ _ _, .inner lrs lrk lrv lrl lrr =>
+          .inner (1 + ls) lk lv ll (.inner (1 + lrs) k v (.inner lrs lrk lrv lrl lrr) .leaf)
+    | .inner rs rk rv rl rr =>
+      if rs > delta * ls then
+        match rl, rr with
+        | .inner rls rlk rlv rll rlr, .inner rrs _ _ _ _ =>
+            if rls < ratio * rrs then
+              .inner (1 + ls + rs) rk rv (.inner (1 + ls + rls) k v l rl) rr
+            else
+              .inner (1 + ls + rs) rlk rlv (.inner (1 + ls + rll.size) k v l rll)
+                (.inner (1 + rrs + rlr.size) rk rv rlr rr)
+        | inner _ _ _ _ _, .leaf => panic! "balanceSlow input was not balanced"
+        | .leaf, _ => panic! "balanceSlow input was not balanced"
+      else if ls > delta * rs then
+        match ll, lr with
+        | .inner lls _ _ _ _, .inner lrs lrk lrv lrl lrr =>
+            if lrs < ratio * lls then
+              .inner (1 + ls + rs) lk lv ll (.inner (1 + rs + lrs) k v lr r)
+            else
+              .inner (1 + ls + rs) lrk lrv (.inner (1 + lls + lrl.size) lk lv ll lrl)
+                (.inner (1 + rs + lrr.size) k v lrr r)
+        | inner _ _ _ _ _, .leaf => panic! "balanceSlow input was not balanced"
+        | .leaf, _ => panic! "balanceSlow input was not balanced"
+      else
+        .inner (1 + ls + rs) k v l r
+
+@[simp]
+theorem balancedAtRoot_zero_zero : BalancedAtRoot 0 0 := by
+  simp only [BalancedAtRoot]; omega
+
+@[simp]
+theorem balancedAtRoot_zero_one : BalancedAtRoot 0 1 := by
+  simp only [BalancedAtRoot]; omega
+
+@[simp]
+theorem balancedAtRoot_one_zero : BalancedAtRoot 1 0 := by
+  simp only [BalancedAtRoot]; omega
+
+@[simp]
+theorem balancedAtRoot_one_one : BalancedAtRoot 1 1 := by
+  simp only [BalancedAtRoot, delta]; omega
+
+@[simp]
+theorem balancedAtRoot_two_one : BalancedAtRoot 2 1 := by
+  simp only [BalancedAtRoot, delta]; omega
+
+@[simp]
+theorem balancedAtRoot_one_two : BalancedAtRoot 1 2 := by
+  simp only [BalancedAtRoot, delta]; omega
+
+theorem balanced_one_leaf_leaf {k : α} {v : β k} : (inner 1 k v leaf leaf).Balanced :=
+  balanced_inner_iff.2 ⟨.leaf, .leaf, by simp [size_leaf], by simp [size_leaf]⟩
+
+theorem balancedAtRoot_zero_iff {n : Nat} : BalancedAtRoot 0 n ↔ n ≤ 1 := by
+  simp only [BalancedAtRoot]; omega
+
+theorem balancedAtRoot_zero_iff' {n : Nat} : BalancedAtRoot n 0 ↔ n ≤ 1 := by
+  simp only [BalancedAtRoot]; omega
+
+theorem Balanced.one_le {sz k v l r} : (Impl.inner sz k v l r : Impl α β).Balanced → 1 ≤ sz := by
+  tree_tac
+
+theorem Balanced.eq {sz k v l r} : (Impl.inner sz k v l r : Impl α β).Balanced → sz = l.size + 1 + r.size
+  | .inner _ _ _ h => h
+
+theorem Balanced.left {sz k v l r} : (Impl.inner sz k v l r : Impl α β).Balanced → l.Balanced
+  | .inner h _ _ _ => h
+
+theorem Balanced.right {sz k v l r} : (Impl.inner sz k v l r : Impl α β).Balanced → r.Balanced
+  | .inner _ h _ _ => h
+
+theorem Balanced.at_root {sz k v l r} : (Impl.inner sz k v l r : Impl α β).Balanced →
+    BalancedAtRoot l.size r.size
+  | .inner _ _ h _ => h
+
+theorem BalancedAtRoot.symm {l r : Nat} : BalancedAtRoot l r → BalancedAtRoot r l := by
+  tree_tac
+
+theorem BalancedAtRoot.erase_left {l l' r : Nat} : BalancedAtRoot l r → l - 1 ≤ l' → l' ≤ l →
+    BalanceLErasePrecond r l' := by tree_tac
+
+theorem BalancedAtRoot.erase_right {l r r' : Nat} : BalancedAtRoot l r → r - 1 ≤ r' → r' ≤ r →
+    BalanceLErasePrecond l r' :=
+  fun h h₁ h₂ => h.symm.erase_left h₁ h₂
+
+theorem BalancedAtRoot.adjust_left {l l' r : Nat} : BalancedAtRoot l r → l - 1 ≤ l' → l' ≤ l + 1 →
+    BalanceLErasePrecond l' r ∨ BalanceLErasePrecond r l' := by tree_tac
+
+theorem BalancedAtRoot.adjust_right {l r r' : Nat} : BalancedAtRoot l r → r - 1 ≤ r' → r' ≤ r + 1 →
+    BalanceLErasePrecond l r' ∨ BalanceLErasePrecond r' l :=
+  fun h h₁ h₂ => h.symm.adjust_left h₁ h₂ |>.symm
+
+theorem balanceLErasePrecond_zero_iff {n : Nat} : BalanceLErasePrecond 0 n ↔ n ≤ 1 := by
+  tree_tac
+
+theorem balanceLErasePrecond_zero_iff' {n : Nat} : BalanceLErasePrecond n 0 ↔ n ≤ 3 := by
+  tree_tac
+
+theorem omega_fact_1 {n m : Nat} (h₂ : n + 1 + m ≤ 3) (h₃ : 1 ≤ n) (h₄ : 1 ≤ m) :
+    n = 1 ∧ m = 1 := by omega
+
+theorem omega_fact_2 {ls rls rrs : Nat} (h₁ : rls < 2 * rrs)
+    (h₂ : BalanceLErasePrecond (rls + 1 + rrs) ls) (h₃ : 1 ≤ ls) : rls ≤ 3 * ls := by
+  dsimp only [tree_tac] at *
+  omega
+
+/-- Constructor for an inner node with the correct size. -/
+@[tree_tac]
+def bin (k : α) (v : β k) (l r : Impl α β) : Impl α β :=
+  .inner (l.size + 1 + r.size) k v l r
+
+/-- A single left rotation. -/
+@[tree_tac]
+def singleL (k : α) (v : β k) (l : Impl α β) (rk : α) (rv : β rk) (rl rr : Impl α β) : Impl α β :=
+  bin rk rv (bin k v l rl) rr
+
+/-- A single right rotation. -/
+@[tree_tac]
+def singleR (k : α) (v : β k) (lk : α) (lv : β lk) (ll lr : Impl α β) (r : Impl α β) : Impl α β :=
+  bin lk lv ll (bin k v lr r)
+
+/-- A double left rotation. -/
+@[tree_tac]
+def doubleL (k : α) (v : β k) (l : Impl α β) (rk : α) (rv : β rk) (rlk : α) (rlv : β rlk)
+    (rll rlr : Impl α β) (rr : Impl α β) : Impl α β :=
+  bin rlk rlv (bin k v l rll) (bin rk rv rlr rr)
+
+/-- A double right rotation. -/
+@[tree_tac]
+def doubleR (k : α) (v : β k) (lk : α) (lv : β lk) (ll : Impl α β) (lrk : α) (lrv : β lrk)
+    (lrl lrr : Impl α β) (r : Impl α β) : Impl α β :=
+  bin lrk lrv (bin lk lv ll lrl) (bin k v lrr r)
